\documentclass{homework}
\usepackage{ dsfont }

\name{Timothy Devon Morris}
\course{EC En 671}
\term{Fall 2018}
\hwnum{1}

\begin{document}

\begin{problem}[2-6]
  Let $(X,d)$ be a metric space. Show that
  \[d_m(x,y) = min(1, d(x,y))\]
  is a metric on $X$
\end{problem}

\begin{solution}
  It is sufficient to show that $d_m$ satisfies the 4 axioms of a metric
  \begin{parts}
    \part 
    M1. 
    \[d_m(x,y) = min(1, d(x,y)) = min(1, d(y,x)) = d_m(y,x)\]
    \part
    M2.
    \[d_m(x,y) = min(1, d(x,y)) \geq 0\]
    Since both $1 \geq 0$, $d(x,y) \geq 0$.
    \part
    M3.
    \[d_m(x,y) = min(1, d(x,y)) = 0 \iff x = y\]
    Since $1 \neq 0$.
    \part
    M4.
    \[d_m(x,z) = min(1, d(x,y)) \leq min(1, d(x,y) + d(y,z))\] 
    by definition. Thus we have that
    \[d_m(x,z) \leq min(1, d(x,y)) + min(1, d(y,z)) = d_m(x,y) + d_m(y,z)\]
  \end{parts}

\end{solution}

\begin{problem}[2-7]
    Define the sequences $\mathbf{x}$, $\mathbf{y}$ by
    \[x_n = \frac{1}{n + 1} \quad y_n = \frac{n}{n + 1}\]
    Show that $d_{\infty}(\mathbf{x},\mathbf{y}) > |x_n - y_n|$ for $n\geq1$.
\end{problem}

\begin{solution}
  We first note that
  \[d_{\infty}(\mathbf{x},\mathbf{y}) = \sup_n \big\lvert\frac{1}{n+1} - \frac{n}{n+1}\big\rvert = \sup_n\frac{n - 1}{n+1} = 1\]
  We also see that 
  \[1 > \frac{n - 1}{n + 1} \quad \forall n \geq 1\]
\end{solution}

\begin{problem}[2-30]
  Let $S$ denote the subset  of all solutions to the following differential equation defined of $C^3[0, \infty)$
  \[ \frac{d^3x}{dt^3} + b\frac{d^2x}{dt^2} + c\frac{dx}{dt} + dx = 0\]
  Show that $S$ is a linear subspace of $C^3[0, \infty)$
\end{problem}

\begin{solution}
  Asssume that $x,y \in S$. It is sufficient to show that $\alpha x + \beta y \in S$ for $\alpha, \beta \in \mathds{R}$.
  Since, the derivative is a linear operator, the proof is straight-forward.

  $
  \begin{aligned}
    &\frac{d^3}{dt^3}(\alpha x + \beta y) + b\frac{d^2}{dt^2}(\alpha x + \beta y) + c\frac{d}{dt}(\alpha x + \beta y) + d(\alpha x + \beta y) = \\
    &\frac{d^3}{dt^3}(\alpha x) + b\frac{d^2}{dt^2}(\alpha x) + c\frac{d}{dt}(\alpha x) + d(\alpha x) + \frac{d^3}{dt^3}(\beta y) + b\frac{d^2}{dt^2}(\beta y) + c\frac{d}{dt}(\beta y) + d(\beta y) = \\
    &\alpha\frac{dx^3}{dt^3} + \alpha b\frac{dx^2}{dt^2} + \alpha c\frac{d}{dt} + \alpha dx + \beta \frac{dy^3}{dt^3} + \beta b\frac{dy^2}{dt^2} + c\frac{dy}{dt} + \beta d y = \\
    &\alpha\left(\frac{d^3x}{dt^3} + b\frac{d^2x}{dt^2} + c\frac{dx}{dt} + dx\right) + \beta\left(\frac{d^3y}{dt^3} + b\frac{d^2y}{dt^2} + c\frac{dy}{dt} + dy\right) = \\
    &\alpha 0 + \beta 0 = 0
  \end{aligned}
  $
  Where the second to last line follows from the definition of $S$.

\end{solution}

\end{document}
