\documentclass{homework}
\usepackage{ dsfont }
\usepackage{ mathtools }
\usepackage{ commath }
\usepackage[final]{ pdfpages }

\name{Timothy Devon Morris}
\course{EC En 671}
\term{Fall 2018}
\hwnum{5}

\begin{document}
\begin{problem}[4-1]
  Write the differential equation
  \[\dddot{x}(t) - 2\ddot{x}(t) - \dot{x}(t) = b(t)\]
  in operator form
\end{problem}

\begin{solution}
  Let 
  \[ A = \frac{d^3}{dt^3} - 2 \frac{d^2}{dt^2} - \frac{d}{dt} \]
  Then we have the equation
  \[ Ax(t) = b(t)\]
\end{solution}

\begin{problem}[4-4]
  Determine the $l_1,l_2,$ Frobenius, and $l_{\infty}$ norms of the following matrices
  \[ A_1 =
    \begin{bmatrix}
      4 & 3 \\
      3 & 6
    \end{bmatrix}
    \quad 
    A_1 =
    \begin{bmatrix}
      1 & 2 \\
      3 & 0
    \end{bmatrix}
    \quad
    A_1 =
    \begin{bmatrix}
      1 & 2 \\
      0 & 1
    \end{bmatrix}
  \]
\end{problem}

\begin{solution}
  $A_1$
  \[ l_1: 9 \quad l_2: 8.1622 \quad \text{Frobenius}: \sqrt{70} \quad l_\infty: 9\]
  $A_2$
  \[ l_1: 4 \quad l_2: 3.2566 \quad \text{Frobenius}: \sqrt{14} \quad l_\infty: 3\]
  $A_3$
  \[ l_1: 3 \quad l_2: 3.2566 \quad \text{Frobenius}: \sqrt{14} \quad l_\infty: 2.414\]
\end{solution}

\begin{problem}[4-10]
  Show that for a square matrix $F$ with $\norm{F}$ and norm satisfying the submultiplicative property,
 \[ \norm{(I - F)^{-1}} \leq \frac{1}{1 - \norm{F}} \]
\end{problem}

\begin{solution}
  Using the neumann series, we have that 
  \[ \norm{(I-F)^{-1}} = \norm{ \sum^{\infty}_{i=0} F^i} \]
  Repeated application of the triangle inequality gives
  \[ \norm{(I-F)^{-1}} \leq \sum^{\infty}_{i=0} \norm{F^i} \]
  The submiltiplicative property gives us
  \[ \norm{(I-F)^{-1}} \leq \sum^{\infty}_{i=0} \norm{F}^i \]
  Once again using the geometric series for scalars, we have
  \[ \norm{(I-F)^{-1}} \leq \frac{1}{1 - \norm{F}} \]
\end{solution}

\begin{problem}[4-15]
  Show that $\norm{A}_F^2 = tr(A^HA)$ 
\end{problem}

\begin{solution}
  We will start with the trace operation
  \[ tr(A^HA) = \sum_{i} [A^HA]_{ii} = \sum_{i} \sum_{k} [A^H]_{ik}[A]_{ki} = \sum_{i} \sum_{k} \bar{a}_{ki} a_{ki} = 
  \sum_{i} \sum_{k} |a_{ki}|^2 = \norm{A}_F^2\]
\end{solution}

\begin{problem}[4-25]
  Show that $(A^*)^{-1} = (A^{-1})^*$ assuming that he inverse exists.
\end{problem}

\begin{solution}
  We begin by noting that in hilbert spaces $A^{**} = A$. Thus we have that
  \[ \langle A^*(A^{-1})^*x, y \rangle = \langle (A^{-1})^*x, Ay\rangle = \langle x, A^{-1}Ay\rangle\ = \langle x, y\rangle\]
  Thus we have that  $A^{*}(A^{-1})^* = I$. Similarly, we have that
  \[ \langle (A^{-1})^*A^*x, y \rangle = \langle (A^*x, A^{-1}y\rangle = \langle x, AA^{-1}y\rangle\ = \langle x, y\rangle\]
  Thus we have that  $(A^{-1})^*A^* = I$. Therefore we have that $(A^*)^{-1} = (A^{-1})^*$.
\end{solution}

\begin{problem}[4-29]
  Determine the 4 fundamental subspaces of 
  \[A =
    \begin{bmatrix}
      1 & 4 \\
      2 & 8 \\
      3 & 12 \\
    \end{bmatrix}
  \]
\end{problem}

\begin{solution}

  $$
  \mathcal{R}(A) = \text{span} \left\{
    \begin{bmatrix}
     1 \\
     2 \\
     3
    \end{bmatrix}
  \right\}
  $$
\end{solution}

\end{document}
